src/program_proof/leasekv/proof.v
@@ -2,6 +2,7 @@ From Perennial.program_proof Require Import grove_prelude.
 From Perennial.program_logic Require Import atomic.
 From Goose.github_com.mit_pdos.gokv Require Import leasekv.
 From Perennial.program_proof.simplepb Require Import renewable_lease.
+From Perennial.program_proof.kv Require Import interface.
 From iris.base_logic.lib Require Import ghost_map.
 
 Module cacheValueC.
@@ -33,46 +34,6 @@ Section proof.
 Context `{!heapGS Σ}.
 Context `{!ghost_mapG Σ string string}.
 Context `{!renewable_leaseG Σ}.
-
-(* KV points-to for the internal kv service *)
-Context {kvptsto_int: string → string → iProp Σ}.
-
-(* Specification of Kv interface. *)
-Definition is_Kv_Put (Put_fn:val) : iProp Σ :=
-  ∀ key value,
-  {{{ True }}}
-  <<< ∀∀ old_value, kvptsto_int key old_value >>>
-    Put_fn #(LitString key) #(LitString value) @ ∅
-  <<< kvptsto_int key value >>>
-  {{{ RET #(); True }}}.
-
-Definition is_Kv_Get (Get_fn:val) : iProp Σ :=
-  ∀ key,
-  {{{ True }}}
-  <<< ∀∀ value, kvptsto_int key value >>>
-    Get_fn #(LitString key) @ ∅
-  <<< kvptsto_int key value >>>
-  {{{ RET #(LitString value); True }}}.
-
-Definition is_Kv_ConditionalPut (CondPut_fn:val) : iProp Σ :=
-  ∀ key expect value,
-  {{{ True }}}
-  <<< ∀∀ old_value, kvptsto_int key old_value >>>
-    CondPut_fn #(LitString key) #(LitString expect) #(LitString value) @ ∅
-  <<< kvptsto_int key (if bool_decide (expect = old_value) then value else old_value) >>>
-  {{{ RET #(LitString (if bool_decide (expect = old_value) then "ok" else "")); True }}}.
-
-Definition is_Kv (k:loc) : iProp Σ :=
-  ∃ Put_fn Get_fn CondPut_fn,
-  "#Hput" ∷ readonly (k ↦[Kv :: "Put"] Put_fn) ∗
-  "#HputSpec" ∷ is_Kv_Put Put_fn ∗
-
-  "#Hget" ∷ readonly (k ↦[Kv :: "Get"] Get_fn) ∗
-  "#HgetSpec" ∷ is_Kv_Get Get_fn ∗
-
-  "#Hcput" ∷ readonly (k ↦[Kv :: "ConditionalPut"] CondPut_fn) ∗
-  "#HcputSpec" ∷ is_Kv_ConditionalPut CondPut_fn
-.
 
 (* FIXME: copies from tutorial proof *)
 Fixpoint string_to_bytes (s:string): list u8 :=
@@ -109,7 +70,10 @@ Definition kvptsto γ key value : iProp Σ :=
   key ↪[γ] {#1/2} value
 .
 
-Definition is_inv γ : iProp Σ :=
+(* KV points-to for the internal kv service *)
+Implicit Types kvptsto_int: string → string → iProp Σ.
+
+Definition is_inv kvptsto_int γ : iProp Σ :=
   inv invN (∃ kvs,
     (* This glues the two maps together *)
     "Hauth" ∷ ghost_map_auth γ 1 kvs ∗
@@ -133,12 +97,12 @@ Definition own_LeaseKv (k:loc) γ : iProp Σ :=
 .
 
 Definition is_LeaseKv (k:loc) γ : iProp Σ :=
-  ∃ mu (kv:loc),
-  "#Hinv" ∷ is_inv γ ∗
+  ∃ mu kvptsto_int (kv:loc),
+  "#Hinv" ∷ is_inv kvptsto_int γ ∗
   "#Hmu" ∷ readonly (k ↦[LeaseKv :: "mu"] mu) ∗
   "#HmuInv" ∷ is_lock nroot mu (own_LeaseKv k γ) ∗
   "#Hkv" ∷ readonly (k ↦[LeaseKv :: "kv"] #kv) ∗
-  "#Hkv_is" ∷ is_Kv kv
+  "#Hkv_is" ∷ is_Kv (kvptsto:=kvptsto_int) kv
 .
 
 Lemma wp_DecodeValue v l :
