src/program_proof/kv/interface.v
@@ -1,0 +1,47 @@
+From Perennial.program_proof Require Import grove_prelude.
+From Perennial.program_logic Require Import atomic.
+From Goose.github_com.mit_pdos.gokv Require Import kv.
+
+Section definitions.
+Context `{!heapGS Σ}.
+(* KV points-to for the internal kv service *)
+Context {kvptsto: string → string → iProp Σ}.
+
+(* Specification of Kv interface. *)
+Definition is_Kv_Put (Put_fn:val) : iProp Σ :=
+  ∀ key value,
+  {{{ True }}}
+  <<< ∀∀ old_value, kvptsto key old_value >>>
+    Put_fn #(LitString key) #(LitString value) @ ∅
+  <<< kvptsto key value >>>
+  {{{ RET #(); True }}}.
+
+Definition is_Kv_Get (Get_fn:val) : iProp Σ :=
+  ∀ key,
+  {{{ True }}}
+  <<< ∀∀ value, kvptsto key value >>>
+    Get_fn #(LitString key) @ ∅
+  <<< kvptsto key value >>>
+  {{{ RET #(LitString value); True }}}.
+
+Definition is_Kv_ConditionalPut (CondPut_fn:val) : iProp Σ :=
+  ∀ key expect value,
+  {{{ True }}}
+  <<< ∀∀ old_value, kvptsto key old_value >>>
+    CondPut_fn #(LitString key) #(LitString expect) #(LitString value) @ ∅
+  <<< kvptsto key (if bool_decide (expect = old_value) then value else old_value) >>>
+  {{{ RET #(LitString (if bool_decide (expect = old_value) then "ok" else "")); True }}}.
+
+Definition is_Kv (k:loc) : iProp Σ :=
+  ∃ Put_fn Get_fn CondPut_fn,
+  "#Hput" ∷ readonly (k ↦[Kv :: "Put"] Put_fn) ∗
+  "#HputSpec" ∷ is_Kv_Put Put_fn ∗
+
+  "#Hget" ∷ readonly (k ↦[Kv :: "Get"] Get_fn) ∗
+  "#HgetSpec" ∷ is_Kv_Get Get_fn ∗
+
+  "#Hcput" ∷ readonly (k ↦[Kv :: "ConditionalPut"] CondPut_fn) ∗
+  "#HcputSpec" ∷ is_Kv_ConditionalPut CondPut_fn
+.
+
+End definitions.
