src/program_proof/lock/lock_proof.v
@@ -1,0 +1,148 @@
+From Perennial.program_proof Require Import grove_prelude std_proof.
+From Goose.github_com.mit_pdos.gokv Require Import lockservice.
+From Perennial.program_proof.kv Require Export interface.
+
+Section lockservice_defns.
+
+(* KV points-to for the internal kv service *)
+Context `{!gooseGlobalGS Σ}.
+
+Record lock_names :=
+  {
+    kvptsto_lock : string → string → iProp Σ
+  }
+.
+End lockservice_defns.
+
+Section lockservice_proof.
+Context `{!heapGS Σ}.
+Definition lock_inv γ key R : iProp Σ :=
+  ∃ b : bool, kvptsto_lock γ key (if b then "1" else "") ∗ if b then True else R.
+
+Context (N: namespace).
+
+Definition is_lock `{invGS Σ} γ key R :=
+  inv N (lock_inv γ key R).
+
+Lemma lock_alloc `{invGS Σ} γ E key R :
+  kvptsto_lock γ key "" -∗ R ={E}=∗ is_lock γ key R.
+Proof.
+  iIntros "Hkv HR".
+  iMod (inv_alloc _ _ (lock_inv γ key R) with "[Hkv HR]").
+  { iNext. iExists false. iFrame. }
+  eauto.
+Qed.
+
+Definition is_LockClerk (ck:loc) γ : iProp Σ :=
+  ∃ (kvCk : loc),
+    "#Hkv" ∷ readonly (ck ↦[LockClerk :: "kv"] #kvCk) ∗
+    "#Hkv_is" ∷ is_Kv (kvptsto:=kvptsto_lock γ) kvCk.
+
+Lemma wp_MakeLockClerk kvCk γ :
+  {{{
+        is_Kv (kvptsto:=kvptsto_lock γ) kvCk
+  }}}
+    MakeLockClerk #kvCk
+  {{{
+       (ck:loc), RET #ck; is_LockClerk ck γ
+  }}}
+.
+Proof.
+  iIntros (Φ) "#Hkv_is HΦ".
+  rewrite /MakeLockClerk.
+  wp_lam.
+  iApply wp_fupd.
+  wp_pures.
+  wp_apply wp_allocStruct; first val_ty.
+  iIntros (?) "Hl".
+  iDestruct (struct_fields_split with "Hl") as "HH".
+  iNamed "HH".
+  iMod (readonly_alloc_1 with "kv") as "#Hkv".
+  iApply "HΦ". iModIntro.
+  repeat iExists _. iFrame "∗#".
+Qed.
+
+Lemma wp_LockClerk__Lock ck key γ R :
+  {{{
+       is_LockClerk ck γ ∗ is_lock γ key R
+  }}}
+    LockClerk__Lock #ck #(str key)
+  {{{
+       RET #(); R
+  }}}
+.
+Proof.
+  iIntros (Φ) "(#Hck&#Hlock) HΦ".
+  wp_lam.
+  wp_pures.
+  wp_apply (wp_forBreak_cond' with "HΦ").
+  iModIntro. iIntros "HΦ".
+  wp_pure1_credit "Hlc".
+  wp_pures.
+  iNamed "Hck".
+  wp_loadField.
+  iNamed "Hkv_is".
+  wp_loadField.
+  wp_apply ("HcputSpec" with "[//]").
+  rewrite /is_lock.
+  replace (⊤ ∖ ∅) with (⊤ : coPset) by set_solver+.
+  iInv "Hlock" as "Hlock_inner" "Hclo".
+  iMod (lc_fupd_elim_later with "Hlc Hlock_inner") as "Hlock_inner".
+  iDestruct "Hlock_inner" as (?) "(Hk&HR)".
+  iApply ncfupd_mask_intro.
+  { solve_ndisj. }
+  iIntros "Hmask".
+  iExists _. iFrame "Hk".
+  iIntros "Hk".
+  iMod "Hmask".
+  destruct b.
+  - rewrite bool_decide_false //.
+    iMod ("Hclo" with "[HR Hk]").
+    { iExists true. iFrame. }
+    iModIntro. iIntros "Hck". wp_pures. iModIntro. iLeft.
+    iSplit; first by eauto.
+    iFrame "HΦ".
+  - rewrite bool_decide_true //.
+    iMod ("Hclo" with "[Hk]").
+    { iExists true. iFrame. }
+    iModIntro. iIntros "Hck". wp_pures. iModIntro. iRight.
+    iSplit; first by eauto.
+    wp_pures. iModIntro. iApply "HΦ". iFrame.
+Qed.
+
+Lemma wp_LockClerk__Unlock ck key γ R :
+  {{{
+       is_LockClerk ck γ ∗ is_lock γ key R ∗ R
+  }}}
+    LockClerk__Unlock #ck #(str key)
+  {{{
+       RET #(); True
+  }}}
+.
+Proof.
+  iIntros (Φ) "(#Hck&#Hlock&HR) HΦ".
+  wp_lam.
+  wp_pure1_credit "Hlc".
+  iNamed "Hck".
+  wp_loadField.
+  iNamed "Hkv_is".
+  wp_loadField.
+  wp_apply ("HputSpec" with "[//]").
+  rewrite /is_lock.
+  replace (⊤ ∖ ∅) with (⊤ : coPset) by set_solver+.
+  iInv "Hlock" as "Hlock_inner" "Hclo".
+  iMod (lc_fupd_elim_later with "Hlc Hlock_inner") as "Hlock_inner".
+  iDestruct "Hlock_inner" as (?) "(Hk&_)".
+  iApply ncfupd_mask_intro.
+  { solve_ndisj. }
+  iIntros "Hmask".
+  iExists _. iFrame "Hk".
+  iIntros "Hk".
+  iMod "Hmask".
+  iMod ("Hclo" with "[HR Hk]").
+  { iExists false. iFrame. }
+  iModIntro. iIntros "Hck".
+  wp_pures. by iApply "HΦ".
+Qed.
+
+End lockservice_proof.
